LambdaS5/coq/LjsRulesCorrectSpecFuns.v
@@ -1,0 +1,416 @@
+Generalizable All Variables.
+Set Implicit Arguments.
+Require Import JsNumber.
+Require Import LjsShared.
+Require Import Utils.
+Require Import LjsRulesCorrectDefinitions.
+Require Import LjsRulesCorrectCommon.
+Import ListNotations.
+Open Scope list_scope.
+Open Scope string_scope.
+
+Implicit Type A B : Type.
+Implicit Type s : string.
+Implicit Type n : number.
+Implicit Type i : L.id.
+Implicit Type st : L.store.
+Implicit Type e : L.expr.
+Implicit Type v : L.value.
+Implicit Type o : L.out.
+Implicit Type c : L.ctx.
+Implicit Type ptr : L.object_ptr.
+Implicit Type obj : L.object.
+Implicit Type re : L.result.
+Implicit Type r : L.res.
+Implicit Type props : L.object_props.
+
+Implicit Type jst : J.state.
+Implicit Type je : J.expr.
+Implicit Type jt : J.stat.
+Implicit Type jee : J.ext_expr.
+Implicit Type jet : J.ext_stat.
+Implicit Type jes : J.ext_spec.
+Implicit Type jc : J.execution_ctx.
+Implicit Type jo : J.out.
+Implicit Type jr : J.res.
+Implicit Type jv : J.value.
+Implicit Type jptr : J.object_loc.
+Implicit Type jobj : J.object.
+Implicit Type jrv : J.resvalue.
+Implicit Type jref : J.ref.
+Implicit Type jl : J.label.
+Implicit Type jer : J.env_record.
+Implicit Type jeptr : J.env_loc.
+Implicit Type jder : J.decl_env_record.
+Implicit Type jprops : J.object_properties_type.
+Implicit Type jlenv : J.lexical_env.
+
+(** ** Lemmas about operators *)
+
+(* TODO *)
+
+(** ** Lemmas about the environment *)
+
+(* TODO *)
+
+(** ** Lemmas about specification functions *)
+
+Lemma make_native_error_lemma : forall BR k jst jc c st st' jv1 jv2 v1 v2 r,
+    L.red_exprh k c st 
+       (L.expr_app_2 LjsInitEnv.privMakeNativeError [v1; v2]) 
+       (L.out_ter st' r) ->
+    state_invariant BR jst jc c st ->
+    (v2 = L.value_undefined \/ exists s, v2 = L.value_string s) ->
+    value_related BR jv1 v1 ->
+    value_related BR jv2 v2 ->
+    concl_ext_expr_value BR jst jc c st st' r (J.spec_build_error jv1 jv2) 
+        (fun jv => exists jptr, jv = J.value_object jptr).
+Proof.
+    introv Hlred Hinv Hv Hvrel1 Hvrel2. 
+    inverts red_exprh Hlred; tryfalse.
+    ljs_apply.
+    repeat ljs_autoforward.
+    destruct_hyp Hv;
+    repeat ljs_autoforward.
+    inverts Hvrel2.
+    jauto_js 12.
+    (* has message *)
+    inv_ljs;
+    binds_inv. (* TODO *) simpls. false. rewrite binds_empty_eq in H8. eauto.
+    repeat ljs_autoforward.
+    inv_ljs; binds_inv. 
+    repeat ljs_autoforward.
+    rew_bag_simpl. 
+    simpls.
+    binds_inv.
+    inverts Hvrel2.
+    unfold_concl. do 3 eexists. splits. 
+    jauto_js 15.
+    jauto_js.
+    eapply state_invariant_next_fresh_commute_object_preserved.
+    rew_bag_simpl.
+    eapply state_invariant_new_object_preserved.
+    eauto_js. eauto_js.
+    eauto_js 15.
+    eauto_js 7.
+    jauto_js 8.
+    simpls. false. prove_bag 7.
+Qed.
+
+Lemma priv_js_error_lemma : forall k c st v st' r,
+    L.red_exprh k c st (L.expr_app_2 LjsInitEnv.privJSError [v]) (L.out_ter st' r) ->
+    exists obj,
+    r = L.res_value (L.value_object (fresh st)) /\
+    st' = st \(fresh st := obj) /\
+    js_exn_object obj v.
+Proof.
+    introv Hlred.
+    inverts red_exprh Hlred; tryfalse.
+    ljs_apply.
+    repeat ljs_autoforward.
+    jauto_js.
+Qed.
+
+Lemma native_error_lemma : forall BR k jst jc c st st' jne ptr v r,
+    L.red_exprh k c st 
+        (L.expr_app_2 LjsInitEnv.privNativeError [L.value_object ptr; v]) 
+        (L.out_ter st' r) ->
+    state_invariant BR jst jc c st ->
+    (v = L.value_undefined \/ exists s, v = L.value_string s) -> (* TODO error messages in jscert *)
+    fact_js_obj (J.object_loc_prealloc (J.prealloc_native_error_proto jne)) ptr \in BR ->
+    concl_ext_expr_value BR jst jc c st st' r (J.spec_error jne) (fun _ => False).
+Proof.
+    introv Hlred Hinv Hv Hbr.
+    inverts red_exprh Hlred; tryfalse.
+    ljs_apply.
+    ljs_state_invariant_after_apply.
+    repeat ljs_autoforward.
+    destruct_hyp Hv;
+    forwards Hx : make_native_error_lemma H0; (destr_concl || jauto_js). (* TODO *)
+    res_related_invert.
+    repeat inv_fwd_ljs.
+    forwards Hy : priv_js_error_lemma. eassumption. destruct_hyp Hy.
+    repeat inv_fwd_ljs.
+    resvalue_related_invert.
+    (* debug *) unfold_concl. jauto_set. eauto_js. eauto_js. 
+        debug eauto 8 with js_ljs bag typeclass_instances nocore xcore.
+    jauto_js 8. 
+    ljs_handle_abort.
+    skip. (* TODO overspecification in jscert - https://github.com/resource-reasoning/jscert_dev/issues/14 *)
+    skip.
+Qed.
+
+Lemma type_error_lemma : forall BR k jst jc c st st' v r,
+    L.red_exprh k c st 
+        (L.expr_app_2 LjsInitEnv.privTypeError [v]) 
+        (L.out_ter st' r) ->
+    (v = L.value_undefined \/ exists s, v = L.value_string s) ->
+    state_invariant BR jst jc c st ->
+    concl_ext_expr_value BR jst jc c st st' r (J.spec_error J.native_error_type) (fun _ => False).
+Proof.
+    introv Hlred Hv Hinv.
+    inverts red_exprh Hlred; tryfalse.
+    ljs_apply.
+    ljs_state_invariant_after_apply.
+    repeat ljs_autoforward.
+    forwards Hx : native_error_lemma; try eassumption.
+    eapply state_invariant_prealloc_in_ctx_lemma. eassumption. eassumption. 
+        repeat (eapply Mem_here || eapply Mem_next). (* TODO *)
+    destr_concl; tryfalse.
+    ljs_handle_abort.
+Qed.
+
+(** *** spec_expr_get_value_conv spec_to_boolean 
+    It corresponds to [to_bool] in the desugaring. *)
+
+Lemma red_spec_to_boolean_unary_ok : forall k,
+    th_ext_expr_unary k LjsInitEnv.privToBoolean J.spec_to_boolean 
+        (fun jv => exists b, jv = J.value_prim (J.prim_bool b)).
+Proof.
+    introv Hinv Hvrel Hlred.
+    inverts red_exprh Hlred; tryfalse.
+
+    ljs_apply.
+
+    repeat ljs_autoforward. 
+
+    inverts Hvrel; try injects; jauto_js.
+Qed.
+
+Lemma red_spec_to_number_unary_ok : forall k,
+    th_ext_expr_unary k LjsInitEnv.privToNumber J.spec_to_number
+        (fun jv => exists n, jv = J.value_prim (J.prim_number n)).
+Proof.
+    introv Hinv Hvrel Hlred.
+    inverts red_exprh Hlred; tryfalse.
+    ljs_apply.
+    ljs_state_invariant_after_apply.
+(* TODO *)
+Admitted.
+
+(* TODO move *)
+Ltac decide_stx_eq := 
+    match goal with
+    | H : context[decide (L.stx_eq ?v1 ?v2)] |- _ => 
+        let EQ := fresh "EQ" in
+        case_if_on (decide (L.stx_eq v1 v2)) as EQ;
+        [applys_to EQ eq_true_r; rew_refl in EQ; try solve [inverts EQ]
+        |applys_to EQ eq_false_r; rew_refl in EQ; try solve [false; apply EQ; jauto_js]]
+    end.
+
+Ltac invert_stx_eq :=
+    match goal with
+    | H : L.stx_eq _ _  |- _ => inverts H
+    end. 
+
+Lemma red_spec_to_object_ok : forall k,
+    th_ext_expr_unary k LjsInitEnv.privToObject J.spec_to_object
+        (fun jv => exists jptr, jv = J.value_object jptr).
+Proof.
+    introv Hinv Hvrel Hlred.
+    inverts red_exprh Hlred; tryfalse.
+    ljs_apply.
+    ljs_state_invariant_after_apply.
+    repeat (ljs_autoforward || decide_stx_eq).
+    (* null *)
+    destruct Hvrel; invert_stx_eq.
+    forwards Hx : type_error_lemma. eassumption. iauto. eauto_js.
+    destr_concl; tryfalse.
+    jauto_js.
+    (* undefined *)
+    destruct Hvrel; invert_stx_eq.
+    forwards Hx : type_error_lemma. eassumption. iauto. eauto_js.
+    destr_concl; tryfalse.
+    jauto_js.
+    (* object *)
+    destruct Hvrel; invert_stx_eq.
+    jauto_js.
+    (* string *)
+    destruct Hvrel; invert_stx_eq.
+    skip. (* TODO *)
+    (* number *)
+    destruct Hvrel; invert_stx_eq.
+    inverts red_exprh H7. (* TODO *)
+    ljs_apply.
+    repeat ljs_autoforward.
+    jauto_js 8.
+    (* boolean *)
+    destruct Hvrel; invert_stx_eq.
+    inverts red_exprh H7. (* TODO *)
+    ljs_apply.
+    repeat ljs_autoforward.
+    jauto_js 8.
+    (* impossible *)
+    destruct Hvrel; false; eauto_js.
+Qed.
+
+Lemma red_spec_to_boolean_ok : forall k je, 
+    ih_expr k ->
+    th_spec k (E.to_bool (js_expr_to_ljs je))
+              (J.spec_expr_get_value_conv J.spec_to_boolean je) 
+              (fun _ _ _ _ _ r jv => exists b, jv = J.value_prim (J.prim_bool b) /\ 
+                  r = L.res_value (L.value_bool b)).
+Proof.
+    introv IHe Hinv Hlred.
+    repeat ljs_autoforward.
+
+    destr_concl; try ljs_handle_abort.
+
+    repeat inv_internal_fwd_ljs.
+    forwards_th red_spec_to_boolean_unary_ok.
+
+    destr_concl.
+    res_related_invert.
+    resvalue_related_invert.
+    jauto_js. left. jauto_js.
+    jauto_js. right. jauto_js.
+Qed.
+
+Lemma new_env_record_object_lemma : forall BR k c st jlenv v jptr ptr b st' r,
+    lexical_env_related BR jlenv v ->
+    value_related BR (J.value_object jptr) (L.value_object ptr) ->
+    L.red_exprh k c st (L.expr_app_2 LjsInitEnv.privnewObjEnvRec 
+        [v; L.value_object ptr; L.value_bool b]) (L.out_ter st' r) ->
+    exists obj,
+    st' = st \(fresh st := obj) /\
+    r = L.res_value (L.value_object (fresh st)) /\
+    binds (L.object_internal obj) "parent" v /\
+    env_record_related BR (J.env_record_object jptr b) obj.
+Proof.
+    introv Hlrel Hvrel Hlred.
+    inverts Hvrel.
+    inverts red_exprh Hlred.
+    ljs_apply.
+    repeat ljs_autoforward.
+    eexists.
+    splits.
+    reflexivity.
+    reflexivity.
+    prove_bag.
+    econstructor;
+    prove_bag 8.
+Qed.
+
+Lemma state_invariant_new_env_record_object_lemma : forall BR k jst jc c st v jptr ptr b st' r,
+    L.red_exprh k c st (L.expr_app_2 LjsInitEnv.privnewObjEnvRec 
+        [v; L.value_object ptr; L.value_bool b]) (L.out_ter st' r) ->
+    binds c "$context" v ->
+    value_related BR (J.value_object jptr) (L.value_object ptr) ->
+    state_invariant BR jst jc c st ->
+    exists obj,
+    st' = st \(fresh st := obj) /\
+    r = L.res_value (L.value_object (fresh st)) /\
+    state_invariant (\{fact_ctx_parent (fresh st) v} \u \{fact_js_env (fresh jst) (fresh st)} \u BR) 
+        (J.state_next_fresh (jst \(fresh jst := J.env_record_object jptr b))) 
+        (J.execution_ctx_with_lex jc (fresh jst::J.execution_ctx_lexical_env jc)) 
+        (c \("$context" := L.value_object (fresh st))) 
+        (st \(fresh st := obj)).
+Proof.
+    introv Hlred Hbinds Hvrel Hinv.
+    asserts Hsub : (BR \c (\{fact_js_env (fresh jst) (fresh st)} \u BR)). 
+        prove_bag 10.
+    asserts Hlerel : (lexical_env_related BR (J.execution_ctx_lexical_env jc) v).
+    solve [eauto using state_invariant_lexical_env_related].
+    forwards Hx : new_env_record_object_lemma; try eauto.
+    destruct_hyp Hx.
+    eexists. splits; try reflexivity.
+    eapply state_invariant_push_context_lemma.
+    eapply lexical_env_related_cons; eauto_js 10. 
+    eauto_js 10. eauto_js 10.
+Qed. 
+
+Lemma decl_env_record_related_empty : forall BR,
+    decl_env_record_related BR \{} \{}.
+Proof.
+    introv. unfolds.
+    intro s.
+    left. splits; prove_bag.
+Qed.
+
+Hint Resolve decl_env_record_related_empty : js_ljs.
+
+(* TODO move *)
+Lemma new_env_record_decl_lemma : forall BR k c st jlenv v st' r,
+    lexical_env_related BR jlenv v ->
+    L.red_exprh k c st (L.expr_app_2 LjsInitEnv.privnewDeclEnvRec [v]) (L.out_ter st' r) ->
+    exists obj,
+    st' = st \(fresh st := obj) /\
+    r = L.res_value (L.value_object (fresh st)) /\
+    binds (L.object_internal obj) "parent" v /\
+    env_record_related BR (J.env_record_decl J.decl_env_record_empty) obj.
+Proof.
+    introv Hlrel Hlred.
+    inverts red_exprh Hlred.
+    ljs_apply.
+    repeat ljs_autoforward.
+    eexists.
+    splits.
+    reflexivity.
+    reflexivity.
+    prove_bag.
+    econstructor; jauto_js.
+Qed.
+
+Lemma state_invariant_new_env_record_decl_lemma : forall BR k jst jc c st v st' r,
+    L.red_exprh k c st (L.expr_app_2 LjsInitEnv.privnewDeclEnvRec [v]) (L.out_ter st' r) ->
+    binds c "$context" v ->
+    state_invariant BR jst jc c st ->
+    exists obj,
+    st' = st \(fresh st := obj) /\
+    r = L.res_value (L.value_object (fresh st)) /\
+    state_invariant (\{fact_ctx_parent (fresh st) v} \u \{fact_js_env (fresh jst) (fresh st)} \u BR) 
+        (J.state_next_fresh (jst \(fresh jst := J.env_record_decl J.decl_env_record_empty))) 
+        (J.execution_ctx_with_lex jc (fresh jst::J.execution_ctx_lexical_env jc)) 
+        (c \("$context" := L.value_object (fresh st))) 
+        (st \(fresh st := obj)).
+Proof.
+    introv Hlred Hbinds Hinv.
+    asserts Hsub : (BR \c (\{fact_js_env (fresh jst) (fresh st)} \u BR)). jauto_js.
+    asserts Hlerel : (lexical_env_related BR (J.execution_ctx_lexical_env jc) v).
+    solve [eauto using state_invariant_lexical_env_related].
+    forwards Hx : new_env_record_decl_lemma; try eauto.
+    destruct_hyp Hx.
+    eexists. splits; try reflexivity.
+    eapply state_invariant_push_context_lemma.
+    eapply lexical_env_related_cons; eauto_js 15.
+    eauto_js 10. eauto_js 10.
+Qed.
+
+(* TODO 
+Lemma decl_env_add_mutable_binding_lemma : forall BR k jst jc c st st' r jeptr ptr obj b jv v s,
+    L.red_exprh k c st (L.expr_app_2 LjsInitEnv.privDeclEnvAddMutableBinding 
+        [L.value_object ptr; L.value_string s; v; L.value_bool b]) (L.out_ter st' r) -> 
+    binds st ptr obj ->
+    state_invariant BR jst jc c st ->
+    value_related BR jv v ->
+    (inr jeptr, ptr) \in BR ->
+    st' = st \(ptr := L.set_object_property obj s (L.attributes_data_of 
+        (L.attributes_data_intro v true false b))) /\
+    r = L.res_value L.value_undefined /\
+    state_invariant BR (J.env_record_write_decl_env jst jeptr s (J.mutability_of_bool b) jv) jc c st'.
+Proof.
+(*
+    introv Hlred Hbinds Hinv.
+    inverts red_exprh Hlred.
+    ljs_apply.
+    repeat ljs_autoforward.
+    cases_decide.
+    repeat ljs_autoforward.
+    solve [inv_ljs].
+*)
+(*
+    repeat ljs_autoforward.
+    inv_ljs.
+    binds_determine. 
+    false. prove_bag.
+    repeat ljs_autoforward. 
+    inv_ljs. 
+    repeat ljs_autoforward.
+    inv_ljs. 
+    repeat ljs_autoforward.
+    simpls.
+
+    binds_inv. false. prove_bag 8.
+*)
+Admitted. (* TODO *)
+*)
